extraction/BluespecFrontEnd/fpga-connectal/Host.bsv
@@ -1,5 +1,6 @@
 import Vector::*;
 import BuildVector::*;
+import RWire::*;
 
 import Proc::*;
 
@@ -45,13 +46,50 @@ module mkFrontEnd#(HostIndication indication) (FrontEnd);
     endmethod
 endmodule
 
+// A frontend wrapper ends
+
+// The closed proc module for giving its synthesis boundary
+
+interface Proc;
+    method Bit#(32) read_toHost_aa;
+    method Bit#(32) read_toHost_a;
+endinterface
+
+(* synthesize *)
+module mkProc (Proc);
+    Wire#(Bit#(32)) val1 <- mkWire();
+    Wire#(Bit#(32)) val2 <- mkWire();
+    Empty procTop <- mkTop (val2._write, val1._write);
+
+    method Bit#(32) read_toHost_aa;
+        return val2;
+    endmethod
+
+    method Bit#(32) read_toHost_a;
+        return val1;
+    endmethod
+
+endmodule
+
+// The closed proc module ends
+
 interface Host;
     interface HostRequest request;
 endinterface
 
 module mkHost#(HostIndication indication) (Host);
     FrontEnd frontEnd <- mkFrontEnd (indication);
-    Empty proc <- mkTop (frontEnd.toHost_aa, frontEnd.toHost_a);
+    Proc proc <- mkProc ();
+
+    rule to_frontend_aa;
+        let val = proc.read_toHost_aa ();
+	frontEnd.toHost_aa(val);
+    endrule
+
+    rule to_frontend_a;
+        let val = proc.read_toHost_a ();
+	frontEnd.toHost_a(val);
+    endrule
 
     interface HostRequest request;
         method Action start ();
